\input{settings.tex}

\begin{document}


\begin{align*}
	\ket{\psi_1} &= \frac{1}{2} \ket{0} \otimes \ket{0} + \frac{\sqrt{3}}{2} \ket{1} \otimes \ket{1}\\
	\ket{\psi_2} &= \frac{1}{4} \ket{0} \otimes \ket{0} + \frac{3}{4} \ket{0} \otimes \ket{1} + \frac{\sqrt{3}}{4} \ket{1} \otimes \ket{0} - \frac{\sqrt{3}}{4} \ket{1} \otimes \ket{1}.
\end{align*}

\begin{align*}
	U \otimes I \ket{\psi_1} = \frac{1}{2} (U \ket{0}) \otimes \ket{0} + \frac{\sqrt{3}}{2} (U \ket{1}) \otimes \ket{1},
\end{align*}
so $U \otimes I \ket{\psi_1} = \ket{\psi_2}$ implies
\begin{align*}
	\frac{1}{2} U \ket{0} &= \frac{1}{4} \ket{0} + \frac{\sqrt{3}}{4} \ket{1}\\
	%
	\frac{\sqrt{3}}{2} U \ket{1} &= \frac{3}{4} \ket{0} - \frac{\sqrt{3}}{4} \ket{1}
\end{align*}
and hence, in the $\{\ket{0}, \ket{1} \}$ basis,
\begin{align*}
	U &=
	\begin{bmatrix}
		\frac{1}{2} & \frac{\sqrt{3}}{2}\\
		\frac{\sqrt{3}}{2} & -\frac{1}{2}
	\end{bmatrix}\\
	%
	U^{-1} &=
	\begin{bmatrix}
		\frac{1}{2} & \frac{\sqrt{3}}{2}\\
		\frac{\sqrt{3}}{2} & -\frac{1}{2}
	\end{bmatrix}.
\end{align*}












\end{document}